Algorithm/Data/Graph.lean
@@ -1,34 +1,53 @@
 
 import Algorithm.Data.Classes.AssocArray
+import Mathlib.Data.List.Nodup
 
 structure Graph where
   V : Type _
-  [instDecidableEqV : DecidableEq V]
-  E : Type _
-  fst' : E → V
-  snd' : E → V
+  [decidableEqV : DecidableEq V]
+  EType : Type _
+  fst' : EType → V
+  snd' : EType → V
   StarList : Type _
-  [instAssocArrayStarList : AssocArray V (List E) StarList]
+  [assocArrayStarList : AssocArray V (List EType) StarList]
   star' : StarList
   costar' : StarList
   fst_star' : ∀ v, ∀ e ∈ AssocArray.get star' v, fst' e = v
   snd_costar' : ∀ v, ∀ e ∈ AssocArray.get costar' v, snd' e = v
+  nodup_star' : ∀ v, (AssocArray.get star' v).Nodup
+  nodup_costar' : ∀ v, (AssocArray.get costar' v).Nodup
+  mem_star'_iff_mem_costar' : ∀ e,
+    e ∈ AssocArray.get star' (fst' e) ↔ e ∈ AssocArray.get costar' (snd' e)
 
 namespace Graph
-variable {g : Graph}
 
-instance : DecidableEq g.V := g.instDecidableEqV
-instance : AssocArray g.V (List g.E) g.StarList := g.instAssocArrayStarList
+attribute [instance] decidableEqV assocArrayStarList
+
+variable {g : Graph}
 -- instance : GetElem g.StarList g.V (List g.E) (fun _ _ ↦ True) := AssocArray.instGetElem
 -- by infer_instance
 
-def E.fst (e : g.E) : g.V := g.fst' e
-def E.snd (e : g.E) : g.V := g.snd' e
+def EType.fst (e : g.EType) : g.V := g.fst' e
+def EType.snd (e : g.EType) : g.V := g.snd' e
 
-def V.star (v : g.V) : List g.E := AssocArray.get g.star' v
-def V.costar (v : g.V) : List g.E := AssocArray.get g.costar' v
+def V.star (v : g.V) : List g.EType := AssocArray.get g.star' v
+def V.costar (v : g.V) : List g.EType := AssocArray.get g.costar' v
 
 lemma fst_star (v : g.V) : ∀ e ∈ v.star, e.fst = v := g.fst_star' v
 lemma snd_costar (v : g.V) : ∀ e ∈ v.costar, e.snd = v := g.snd_costar' v
+
+lemma nodup_star (v : g.V) : v.star.Nodup := g.nodup_star' v
+lemma nodup_costar (v : g.V) : v.costar.Nodup := g.nodup_costar' v
+
+lemma mem_star_iff_mem_costar (e : g.EType) : e ∈ e.fst.star ↔ e ∈ e.snd.costar :=
+  g.mem_star'_iff_mem_costar' e
+
+def E (g : Graph) := {e : g.EType // e ∈ e.fst.star}
+
+def E.fst (e : g.E) : g.V := e.val.fst
+def E.snd (e : g.E) : g.V := e.val.snd
+
+lemma E.mem_star (e : g.E) : e.val ∈ e.fst.star := e.2
+lemma E.mem_costar (e : g.E) : e.val ∈ e.snd.costar := (mem_star_iff_mem_costar _).mp e.2
 
 end Graph
